Sql.v
@@ -1,0 +1,482 @@
+Load "eztactics.v".
+
+Add LoadPath "Listkit" as Listkit.
+
+Require Import Term.
+
+(* To do: Need a "table" form. *)
+Require Import Bool.
+
+Definition is_basic_type T := T = TyBase.
+
+Inductive is_row_type : Ty -> Type :=
+| row_type_wit : forall s t, is_basic_type s -> is_basic_type t -> is_row_type (TyPair s t).
+
+Inductive is_relation_type : Ty -> Type :=
+| relation_type_wit : forall t, is_row_type t -> is_relation_type (TyList t).
+
+Fixpoint is_basic_form B :=
+  match B with
+  | TmIf B1 B2 B3 => is_basic_form B1 && is_basic_form B2 && is_basic_form B3
+  | TmProj b (TmVar x) => true
+  | TmConst => true
+  | _ => false
+  end.
+
+Fixpoint is_row_form R :=
+  match R with
+  | TmPair b1 b2 => is_basic_form b1 && is_basic_form b2
+  | TmVar x => true
+  | _ => false
+  end.
+
+Fixpoint is_filtered_relation Z :=
+  match Z with
+  | TmIf b Z TmNull => is_basic_form b && is_filtered_relation Z
+  | TmSingle R => is_row_form R
+  | TmTable t => true
+  | _ => false
+  end.
+
+Fixpoint is_joined_relation F :=
+  match F with
+  | TmBind (TmTable t) F => is_joined_relation F
+  | _ => is_filtered_relation F
+  end.
+
+Fixpoint is_in_sql_like_sublang M :=
+  match M with
+  | TmUnion M1 M2 => is_in_sql_like_sublang M1 && is_in_sql_like_sublang M2
+  | TmNull => true
+  | _ => is_joined_relation M
+  end.
+
+Require Import Rewrites.
+
+Definition Rewrites M := {N:Term & (M ~> N) }.
+
+Hint Unfold Rewrites.
+
+Definition Normal M := notT (Rewrites M).
+
+Hint Transparent Rewrites Normal.
+
+Lemma Normal_sub_TmPair_1 : forall M N,
+    Normal (TmPair M N) -> Normal M.
+Proof.
+Admitted.
+
+Lemma Normal_sub_TmPair_2 : forall M N,
+    Normal (TmPair M N) -> Normal N.
+Proof.
+Admitted.
+
+Lemma Normal_sub_TmUnion_1 : forall M N,
+    Normal (TmUnion M N) -> Normal M.
+Proof.
+Admitted.
+
+Lemma Normal_sub_TmUnion_2 : forall M N,
+    Normal (TmUnion M N) -> Normal N.
+Proof.
+Admitted.
+
+Lemma Normal_sub_TmBind_1 : forall M N,
+    Normal (TmBind M N) -> Normal M.
+Proof.
+Admitted.
+
+Lemma Normal_sub_TmBind_2 : forall M N,
+    Normal (TmBind M N) -> Normal N.
+Proof.
+Admitted.
+
+Lemma Normal_sub_TmProj : forall b M,
+    Normal (TmProj b M) -> Normal M.
+Proof.
+Admitted.
+
+Lemma Normal_sub_TmSingle : forall M,
+    Normal (TmSingle M) -> Normal M.
+Proof.
+Admitted.
+
+Lemma Normal_sub_TmApp_1 : forall L M,
+    Normal (TmApp L M) -> Normal L.
+Proof.
+Admitted.
+
+Lemma Normal_sub_TmApp_2 : forall L M,
+    Normal (TmApp L M) -> Normal M.
+Proof.
+Admitted.
+
+Hint Resolve Normal_sub_TmPair_1 Normal_sub_TmPair_2 Normal_sub_TmUnion_1 Normal_sub_TmUnion_2
+     Normal_sub_TmBind_1 Normal_sub_TmBind_2
+     Normal_sub_TmProj Normal_sub_TmSingle
+     Normal_sub_TmApp_1 Normal_sub_TmApp_2.
+
+Hint Extern 1 (Normal ?M) =>
+match goal with
+| H : Normal (TmPair ?N M) |- _ => eapply Normal_sub_TmPair_2; eauto
+| H : Normal (TmPair M ?N) |- _ => eapply Normal_sub_TmPair_1; eauto
+
+| H : Normal (TmUnion M ?N) |- _ => eapply Normal_sub_TmUnion_1; eauto
+| H : Normal (TmUnion ?N M) |- _ => eapply Normal_sub_TmUnion_2; eauto
+
+| H : Normal (TmBind M ?N) |- _ => eapply Normal_sub_TmBind_1; eauto
+| H : Normal (TmBind ?N M) |- _ => eapply Normal_sub_TmBind_2; eauto
+
+| H : Normal (TmProj ?b M) |- _ => eapply Normal_sub_TmProj; eauto
+| H : Normal (TmSingle M) |- _ => eapply Normal_sub_TmSingle; eauto
+
+| H : Normal (TmApp M ?N) |- _ => eapply Normal_sub_TmApp_1; eauto
+| H : Normal (TmApp ?N M) |- _ => eapply Normal_sub_TmApp_2; eauto
+end.
+
+Axiom var_not_closed: forall x T, notT(Typing nil (TmVar x) T).
+
+Ltac bogus_normal H :=
+  exfalso; apply H; eauto.
+
+(* Note: Missing in the thesis: The inductive premise that M's typing
+   env defines only variables of basic, row or relation type. *)
+
+Require Import Lists.List.
+
+Lemma row_type_in_row_env:
+  forall T env x,
+  (forall s : Ty, In s env -> is_row_type s) ->
+    value T = nth_error env x ->
+    is_row_type T.
+Proof.
+  intros.
+  apply H.
+  eauto using nth_error_In.
+Qed.
+
+Lemma row_env_Normal_forms:
+  forall M T env,
+    Normal M ->
+    (forall s, In s env -> is_row_type s) ->
+    Typing env M T ->
+    (match T return Type with
+     | TyBase => {b : bool & {x : nat & M = TmProj b (TmVar x)}} + (M = TmConst)
+     | TyPair _ _ =>
+       {x : nat & M = TmVar x} + {m : Term & {n : Term & M = TmPair m n}}
+     | TyArr _ _ => {N : Term & M = TmAbs N}
+     | TyList _ =>
+       {T : Ty & {N : Term & M = TmBind (TmTable T) N}} +
+       {M1 & {M2 & M = TmUnion M1 M2}} +
+       {N & M = TmSingle N} +
+       {T : Ty & M = TmTable T} +
+       (M = TmNull)
+    end).
+Proof.
+  induction M; intros T env Normal_M env_typs H; inversion H; subst;
+    (try (solve [split; intros S0 T0 H0; discriminate])).
+
+  - auto.
+  - assert (is_row_type T) by (eauto using row_type_in_row_env).
+    destruct T;
+      try (inversion H0).
+    left; eauto.
+
+  - right; eauto.
+
+  - assert (Normal M) by auto.
+    specialize (IHM (TyPair T t) env H0 env_typs H3).
+    simpl in IHM.
+    destruct IHM as [[x Heq] | [m [n Heq]]].
+    * destruct T; intuition; try discriminate.
+
+      -- subst.
+         left; eexists.
+         eauto.
+
+         (* Hmm, three repeated cases follow... *)
+      -- exfalso.
+         subst M.
+         inversion H3; subst.
+         assert (is_row_type (TyPair (TyPair T1 T2) t)) by (eauto using row_type_in_row_env).
+         inversion H1.
+         inversion H6.
+
+      -- exfalso.
+         subst M.
+         inversion H3; subst.
+         assert (is_row_type (TyPair (TyArr T1 T2) t)) by (eauto using row_type_in_row_env).
+         inversion H1.
+         inversion H6.
+
+      -- exfalso.
+         subst M.
+         inversion H3; subst.
+         assert (is_row_type (TyPair (TyList T) t)) by (eauto using row_type_in_row_env).
+         inversion H1.
+         inversion H6.
+
+    * subst.
+      unfold Normal in H.
+      lapply Normal_M; try easy.
+      unfold Rewrites.
+      eauto.
+
+  - (* The TmProj true case; exactly parallel to the above. Must automate or something...*)
+    assert (Normal M) by auto.
+    specialize (IHM (TyPair s T) env H0 env_typs H3).
+    simpl in IHM.
+    destruct IHM as [[x Heq] | [m [n Heq]]].
+    * destruct T; intuition; try discriminate.
+
+      -- subst.
+         left; eexists.
+         eauto.
+
+      -- exfalso.
+         subst M.
+         inversion H3; subst.
+         assert (is_row_type (TyPair s (TyPair T1 T2))) by (eauto using row_type_in_row_env).
+         inversion H1.
+         inversion H7.
+
+      -- exfalso.
+         subst M.
+         inversion H3; subst.
+         assert (is_row_type (TyPair s (TyArr T1 T2))) by (eauto using row_type_in_row_env).
+         inversion H1.
+         inversion H7.
+
+      -- exfalso.
+         subst M.
+         inversion H3; subst.
+         assert (is_row_type (TyPair s (TyList T))) by (eauto using row_type_in_row_env).
+         inversion H1.
+         inversion H7.
+
+    * subst.
+      unfold Normal in H.
+      lapply Normal_M; try easy.
+      unfold Rewrites.
+      eauto.
+
+  - eauto.
+
+  - exfalso.
+    assert (H0 : Normal M1) by auto.
+    specialize (IHM1 (TyArr a T) env H0 env_typs H2).
+    simpl in IHM1.
+    destruct IHM1 as [N Neq].
+    subst M1.
+    unfold Normal in Normal_M.
+    unfold Rewrites in Normal_M.
+    apply Normal_M.
+    eauto.
+    Unshelve.
+    exact 0.
+
+  - auto.
+  - eauto.
+  - eauto 7.
+  - assert (H0 : Normal M1) by auto.
+    specialize (IHM1 (TyList s) env H0 env_typs H2).
+    simpl in IHM1.
+    destruct IHM1 as [[[[[T [N M1eq]] |
+                         [M11 [M12 M1eq]]] |
+                        [N M1eq]] |
+                       [T M1eq]] |
+                      ?];
+      try (solve [subst; bogus_normal Normal_M]).
+    subst.
+    eauto 7.
+  - eauto.
+Unshelve.
+exact 0.
+Qed.
+
+Inductive is_basic_formi : Term -> Type :=
+| is_basic_formi_1 : forall b1 b2 b3,
+    is_basic_formi b1 -> is_basic_formi b2 -> is_basic_formi b3 -> is_basic_formi (TmIf b1 b2 b3)
+| is_basic_formi_2 : forall b x, is_basic_formi (TmProj b (TmVar x))
+| is_basic_formi_3 : is_basic_formi TmConst
+.
+
+Inductive is_row_formi : Term -> Type :=
+| is_row_formi_1 :
+    forall b1 b2, is_basic_formi b1 -> is_basic_formi b2 -> is_row_formi (TmPair b1 b2)
+| is_row_formi_2 : forall x, is_row_formi (TmVar x)
+.
+
+Inductive is_filtered_relationi : Term -> Type :=
+| is_filtered_relationi_1 :
+    forall b Z,
+      is_basic_formi b -> is_filtered_relationi Z -> is_filtered_relationi (TmIf b Z TmNull)
+| is_filtered_relationi_2 : forall R, is_row_formi R -> is_filtered_relationi (TmSingle R)
+| is_filtered_relationi_3 : forall t, is_filtered_relationi (TmTable t)
+.
+
+Inductive is_joined_relationi : Term -> Type :=
+| is_joined_relationi_1 :
+    forall t F, is_joined_relationi F -> is_joined_relationi (TmBind (TmTable t) F)
+| is_joined_relationi_2 : forall F, is_filtered_relationi F -> is_joined_relationi F
+.
+
+Inductive is_in_sql_like_sublangi : Term -> Type :=
+| is_in_sql_like_sublangi_1 :
+    forall M1 M2,
+      is_in_sql_like_sublangi M1 -> is_in_sql_like_sublangi M2 ->
+      is_in_sql_like_sublangi (TmUnion M1 M2)
+| is_in_sql_like_sublangi_2 :
+    is_in_sql_like_sublangi TmNull
+| is_in_sql_like_sublangi_3 : forall M, is_joined_relationi M -> is_in_sql_like_sublangi M
+.
+
+Hint Constructors is_in_sql_like_sublangi is_joined_relationi is_filtered_relationi is_row_formi is_basic_formi.
+
+Lemma SQL_Normal_forms:
+  forall M T env,
+    Normal M ->
+    (forall s, In s env -> is_row_type s) ->
+    Typing env M T ->
+    (is_basic_type T -> is_basic_formi M) *
+    (is_row_type T -> is_row_formi M) *
+    (is_relation_type T -> is_in_sql_like_sublangi M).
+Proof.
+  induction M; intros T env Normal_M env_typs H;
+    pose (X:=row_env_Normal_forms _ T env Normal_M env_typs H);
+    inversion H; subst T.
+
+  - repeat split; intro Z; inversion Z; eauto.
+
+  - repeat split; intro Z.
+
+    apply row_type_in_row_env in H1; auto.
+    destruct ty; inversion H1; inversion Z.
+    auto.
+    apply row_type_in_row_env in H1; auto.
+    destruct ty; inversion H1; inversion Z.
+
+  - repeat split; intro Z; inversion Z; eauto.
+
+    assert (is_basic_formi M1).
+    { assert (Normal_M1:Normal M1) by auto.
+      apply (IHM1 _ _ Normal_M1 env_typs H2); auto. }
+    assert (is_basic_formi M2).
+    { assert (Normal_M2:Normal M2) by auto.
+      apply (IHM2 _ _ Normal_M2 env_typs H4); auto. }
+    auto.
+
+  - repeat split; intro Z; inversion Z; subst.
+    destruct X as [s | s].
+    destruct s as [b [x eq]].
+    inversion eq.
+    auto.
+
+    inversion s.
+
+    destruct X as [s | s].
+    destruct s as [x eq].
+    inversion eq.
+    destruct s as [m [n eq]].
+    inversion eq.
+    destruct X as [[[[X | X] | X] | X] | X].
+    destruct X as [T [N eq]].
+    discriminate.
+    destruct X as [M1 [M2 eq]].
+    discriminate.
+    destruct X as [N eq].
+    discriminate.
+    destruct X as [T eq].
+    discriminate.
+    discriminate.
+
+  - admit (* Other proj case *).
+
+  - repeat split; intro Z; inversion Z; eauto.
+
+  - subst.
+    assert (Normal M1) by auto.
+    pose (Y := row_env_Normal_forms M1 _ env H0 env_typs H2).
+    simpl in Y.
+    destruct Y as [N eq].
+    subst.
+    bogus_normal Normal_M.
+
+  - repeat split; intro Z; inversion Z; eauto.
+
+  - repeat split; intro Z; inversion Z; eauto.
+
+    subst.
+    assert (Normal M) by auto.
+    specialize (IHM _ _ H0 env_typs H1); destruct IHM as [[? ?] ?].
+    auto.
+
+  - repeat split; intro Z; inversion Z; eauto.
+    assert (Normal M1) by auto.
+    assert (Normal M2) by auto.
+    specialize (IHM1 _ _ H6 env_typs H2); destruct IHM1 as [[? ?] ?].
+    specialize (IHM2 _ _ H7 env_typs H4); destruct IHM2 as [[? ?] ?].
+    apply is_in_sql_like_sublangi_1; auto.
+
+  - repeat split; intro Z; inversion Z; eauto.
+    assert (Normal M1) by auto.
+    assert (Normal M2) by auto.
+    assert (H8 : {t& M1 = TmTable t}).
+    pose (Y := row_env_Normal_forms M1 _ env H6 env_typs H2).
+    simpl in Y.
+    destruct Y as [[[[Y | Y] | Y] | Y] | Y].
+    destruct Y as [T [N eq]]; subst.
+    bogus_normal Normal_M.
+    destruct Y as [M11 [M12 eq]]; subst.
+    bogus_normal Normal_M.
+    destruct Y as [N eq]; subst.
+    bogus_normal Normal_M.
+    destruct Y as [T eq]; subst.
+    eauto.
+    subst.
+    bogus_normal Normal_M.
+    destruct H8 as [T eq]; subst.
+    apply is_in_sql_like_sublangi_3.
+    apply is_joined_relationi_1.
+    assert (is_row_type s).
+    admit (* Need to limit the type of each TmTable somehow! *).
+    assert (H8 : forall r : Ty, In r (s :: env) -> is_row_type r).
+    { intros.
+      apply in_inv in H1.
+      assert (H3 : {s = r} + {In r env}) by admit. (* case analysis on Prop over Set :-( *)
+      destruct H3; subst; auto. }
+    specialize (IHM2 (TyList t) (s :: env) H7 H8 H4).
+    destruct IHM2 as [[IHM2 IHM2'] IHM2''].
+    lapply IHM2''.
+    intros.
+    destruct M2; inversion H1; auto.
+    bogus_normal Normal_M.
+    admit (* Missing a rewrite rule for TmBind (TmTable x) TmNull *).
+    bogus_normal Normal_M.
+    admit (* Missing a rewrite rule for TmBind (TmTable x) (TmUnion x y) *).
+    auto.
+  - repeat split.
+    intro H0; inversion H0.
+    intro H0; inversion H0.
+    intro H0.
+    auto.
+Unshelve. (* ?? *)
+exact 0.
+exact 0.
+Admitted.
+
+
+Lemma SQL_Normal_form:
+  forall M T,
+    Normal M ->
+    Typing nil M T ->
+    is_relation_type T -> is_in_sql_like_sublangi M.
+Proof.
+  intros.
+  lapply (SQL_Normal_forms M T nil H).
+  intros H2.
+  specialize (H2 H0).
+  apply H2; auto.
+  simpl.
+  intuition.
+Qed.
